lean/PuzzleScript/Ids.lean
@@ -15,6 +15,11 @@ structure ObjectId where
   val : Nat
   deriving DecidableEq, Repr, Inhabited
 
+/-- Index into `Game.levels` (playable or message entries). -/
+structure LevelIdx where
+  val : Nat
+  deriving DecidableEq, Repr, Inhabited
+
 instance : Hashable TileIdx where
   hash t := hash t.val
 
@@ -24,8 +29,12 @@ instance : Hashable LayerIdx where
 instance : Hashable ObjectId where
   hash o := hash o.val
 
+instance : Hashable LevelIdx where
+  hash ℓ := hash ℓ.val
+
 /-- Convenience constructors. -/
 def ObjectId.ofNat (n : Nat) : ObjectId := ⟨n⟩
 def LayerIdx.ofNat (n : Nat) : LayerIdx := ⟨n⟩
+def LevelIdx.ofNat (n : Nat) : LevelIdx := ⟨n⟩
 
 end PuzzleScript
